\let\negmedspace\undefined
\let\negthickspace\undefined
\documentclass[journal,12pt,twocolumn]{IEEEtran}
\usepackage{cite}
\usepackage{amsmath,amssymb,amsfonts,amsthm}
\usepackage{algorithmic}
\usepackage{graphicx}
\usepackage{textcomp}
\usepackage{xcolor}
\usepackage{txfonts}
\usepackage{listings}
\usepackage{enumitem}
\usepackage{mathtools}
\usepackage{gensymb}
\usepackage{comment}
\usepackage[breaklinks=true]{hyperref}
\usepackage{tkz-euclide} 
\usepackage{listings}
\usepackage{gvv}                                        
\def\inputGnumericTable{}                                 
\usepackage[latin1]{inputenc}                                
\usepackage{color}                                            
\usepackage{array}                                            
\usepackage{longtable}                                       
\usepackage{calc}                                             
\usepackage{multirow}                                         
\usepackage{hhline}                                           
\usepackage{ifthen}                                           
\usepackage{lscape}

\newtheorem{theorem}{Theorem}[section]
\newtheorem{problem}{Problem}
\newtheorem{proposition}{Proposition}[section]
\newtheorem{lemma}{Lemma}[section]
\newtheorem{corollary}[theorem]{Corollary}
\newtheorem{example}{Example}[section]
\newtheorem{definition}[problem]{Definition}
\newcommand{\BEQA}{\begin{eqnarray}}
\newcommand{\EEQA}{\end{eqnarray}}
\newcommand{\define}{\stackrel{\triangle}{=}}
\theoremstyle{remark}
\newtheorem{rem}{Remark}
\begin{document}
\parindent 0px

\bibliographystyle{IEEEtran}
\vspace{3cm}

\title{Assignment}
\author{EE22BTECH11019 - Dhruv Parashar$^{}$% <-this % stops a space
}
\maketitle
\newpage
\bigskip

\renewcommand{\thefigure}{\theenumi}
\renewcommand{\thetable}{\theenumi}
\textbf{Question:} Find the sum of n terms of an AP where common difference = $d$ using Contour Integration.\\
\solution\\
\\
\begin{tabular}{|p{2cm}|p{2.80cm}|p{2.70cm}|}
    \hline
    Symbol&Value&Description\\ \hline
    $$x(n)$$&$$(x(0)+nd)u(n)$$&$$n^{th}$$ term of an A.P\\ \hline
    $$x(0)$$&$$x(0)$$&$1^{st}$ term of the A.P\\ \hline
    $$d$$&$$d$$&Common difference\\ \hline
    $$u(n)$$&unit step function&$u(n)=0$ \brak {n<0}   $u(n)=1$ \brak {n\geq0}\\ \hline
    $$s(n)$$&$$\sum_{k=0}^{n} x \brak{k}$$&Sum of n terms of an AP\\ \hline
\end{tabular}

\begin{align}
    X \brak{z} &= \sum_{n=-\infty}^{\infty} x \brak{n}   z^{-n}\\
     & = \sum_{n=-\infty}^{\infty}(x(0)+nd)u(n)z^{-n}\\
    U \brak{z} &= \frac{1}{1-z^{-1}},  |z|>1\\
    X \brak{z} & = \frac{x(0)}{1-z^{-1}} + \frac{dz^{-1}}{(1-z^{-1})^{2}}\\
    S\brak{z} &= \sum_{n=-\infty}^{\infty}s(n)z^{-n}\\
    s\brak{n} &= x\brak{n} \ast u\brak{n}\\
    S\brak{z} &= X\brak{z}U\brak{z}\\
     &= \brak{\frac{x(0)}{1-z^{-1}} + \frac{dz^{-1}}{(1-z^{-1})^{2}}}\brak{\frac{1}{1-z^{-1}}}, |z|>1
\end{align}
By performing inverse Z transform on S\brak{z} using contour integration
\begin{align}
   s(n)&=\frac{1}{2\pi j}\oint_{C}S(z) \;z^{n-1} \;dz  \\
   s(n)&=\frac{1}{2\pi j}\oint_{C}\brak{\dfrac{x\brak{0}z^{n-1}}{\brak{1-z^{-1}}^2} + \dfrac{dz^{n-2}}{\brak{1-z^{-1}}^{3}}}\;dz  
\end{align}
For $R_1$ we can observe that the pole has been repeated twice.
\begin{align}
    R&=\frac{1}{\brak {m-1}!}\lim\limits_{z\to a}\frac{d^{m-1}}{dz^{m-1}}\brak {{(z-a)}^{m}f\brak z}\\
    R_1&=\frac{1}{\brak {1}!}\lim\limits_{z\to 1}\frac{d}{dz}\brak {{(z-1)}^{2}\frac{x\brak{0}z^{n+1}}{{(z-1)}^2}}\\
    &=x\brak{0}\brak{n+1}\lim\limits_{z\to 1}\brak{z^n}\\
    &=x\brak{0}\brak{n+1}
\end{align}
For $R_2$ we can observe that the pole has been repeated thrice.
\begin{align}
    R_2&=\frac{1}{\brak {2}!}\lim\limits_{z\to 1}\frac{d^{2}}{dz^{2}}\brak {{(z-1)}^{3}\frac{dz^{n+1}}{{(z-1)}^3}}\\
    &=\frac{d\brak{n+1}}{2}\lim\limits_{z\to 1}\frac{d}{dz}\brak{z^n}\\
    &=\frac{d\brak{n+1}\brak{n}}{2}\lim\limits_{z\to 1}\brak{z^{n-1}}\\
    &=\frac{d\brak{n}\brak{n+1}}{2}\\
    \implies R&= R_1 + R_2\\
    &=x\brak{0}\brak{n+1}+\frac{d\brak{n}\brak{n+1}}{2}
\end{align}
Finally,
\begin{align}
    s\brak{n}&=x\brak{0}\brak{n+1}u\brak{n}+d\brak{\dfrac{{n\brak{n+1}}}{2}}u\brak{n}\\
    &=\dfrac{n+1}{2}\brak{2x\brak{0}+nd}u\brak{n}
\end{align}
\end{document}
